테이블 스키마 자체에, 외부 조건을 넣는 게 맞는건가...

src/ecma335/Nemonuri.Ecma335.Metadata.Heap.fst
@@ -5,6 +5,7 @@ module Te = Nemonuri.Ecma335.Metadata.TableEntry
 module Ter = Nemonuri.Ecma335.Metadata.TableEntry.Refinement
 module S = FStar.Set
 module Ref = Nemonuri.Ref
+module F = FStar.FunctionalExtensionality
 
 open Nemonuri.Ecma335.Metadata.Table
 open FStar.Tactics.Typeclasses
@@ -24,6 +25,11 @@ type string_data = { ref:Ref.t }
 instance emptyable_string : emptyable string_data = {
   is_empty = fun str -> str.ref |> Ref.is_null
 }
+
+type string_heap = table:tablelike Te.t string_data{F.feq table.id_predicate Ter.string_heap_index_predicate}
+
+let is_indexing_empty_string (heap:string_heap) (idx:Ter.string_heap_index) : Tot bool =
+  is_indexing_empty heap idx
 //---|
 
 //--- guid ---
@@ -32,10 +38,9 @@ type guid_data = { ref:Ref.t }
 instance emptyable_guid : emptyable guid_data = {
   is_empty = fun g -> g.ref |> Ref.is_null
 }
+
+type guid_heap = table:tablelike Te.t guid_data{F.feq table.id_predicate Ter.guid_heap_index_predicate}
+
+let is_indexing_null_guid (heap:guid_heap) (idx:Ter.guid_heap_index) : Tot bool =
+  is_indexing_empty heap idx
 //---|
-
-let is_indexing_empty_string (e:Ter.string_heap_index{not (is_null e)}) : Tot bool =
-  false // Todo: be specific
-
-let is_indexing_null_guid (e:guid_heap_index{not (is_null e)}) : Tot bool =
-  false // Todo: be specific
