src/ecma335/Nemonuri.Ecma335.Metadata.TableEntry.Refinement.fst
@@ -2,15 +2,11 @@ module Nemonuri.Ecma335.Metadata.TableEntry.Refinement
 
 module M = Nemonuri.Ecma335.Metadata
 module Te = Nemonuri.Ecma335.Metadata.TableEntry
-module Rf = Nemonuri.Refinement.Tot
-module F = FStar.FunctionalExtensionality
 
-let string_heap_index : Rf.t Te.t = {
-  predicate = F.on Te.t Te.StringHeap?
-}
+let string_heap_index_predicate = Te.StringHeap?
+let string_heap_index = x:Te.t{string_heap_index_predicate x}
 
-let guid_heap_index : Rf.t Te.t = {
-  predicate = F.on Te.t Te.GuidHeap?
-}
+let guid_heap_index_predicate = Te.GuidHeap?
+let guid_heap_index = x:Te.t{guid_heap_index_predicate x}
 
-let assert_string_and_guid_indexes_are_distinct (s:Rf.refine string_heap_index) (g:Rf.refine guid_heap_index) = assert (~(s === g))
+let assert_string_and_guid_indexes_are_distinct (s:string_heap_index) (g:guid_heap_index) = assert (s <> g)
