src/ecma335/Nemonuri.Ecma335.Metadata.ModuleTable.fst
@@ -5,6 +5,7 @@ module Ts = Nemonuri.Ecma335.Metadata.TableSchema
 module L = FStar.List.Tot
 
 (* 1. The Module table shall contain one and only one row [ERROR] *)
+noeq
 type t = {
   v: list Ts.module_schema;
   only_one_row: squash (L.length v == 1)
