src/ecma335/Nemonuri.Ecma335.Metadata.Table.fst
@@ -1,15 +1,14 @@
 module Nemonuri.Ecma335.Metadata.Table
 
 module M = Nemonuri.Ecma335.Metadata
-module Rf = Nemonuri.Refinement.Tot
 
 open FStar.Tactics.Typeclasses
 
 class tablelike (id_t:eqtype) (data_t:Type) =
 {
-  id_domain : Rf.t id_t;
-  get_data : (Rf.refine id_domain) -> data_t
+  id_predicate : id_t -> Tot bool;
+  get_data : x:id_t{id_predicate x} -> data_t
 }
 
 let has_id (#id_t:eqtype) (#data_t:Type) (table: tablelike id_t data_t) (id:id_t) : Tot bool =
-  table.id_domain.predicate id
+  table.id_predicate id
