src/ecma335/Nemonuri.Ecma335.Metadata.TableSchema.fst
@@ -2,6 +2,7 @@ module Nemonuri.Ecma335.Metadata.TableSchema
 module M = Nemonuri.Ecma335.Metadata
 module Te = Nemonuri.Ecma335.Metadata.TableEntry
 module Ter = Nemonuri.Ecma335.Metadata.TableEntry.Refinement
+module Heap = Nemonuri.Ecma335.Metadata.Heap
 
 //--- module ---
 (* https://github.com/stakx/ecma-335/blob/master/docs/ii.22.30-module_0x00.md *)
@@ -12,17 +13,20 @@ module Ter = Nemonuri.Ecma335.Metadata.TableEntry.Refinement
 *)
 
 (* The Module table has the following columns: *)
+noeq
 type module_schema = {
 
+  string_heap: Heap.string_heap;
+  guid_heap: Heap.guid_heap;
   (* - Name (an index into the String heap) *)
   (* 
      2. Name shall index a non-empty string. 
         This string should match exactly any corresponding ModuleRef.Name string that resolves to this module. [ERROR] 
   *)
-  name: x:Te.string_heap_index{not (Te.is_null x) && not (Te.is_indexing_empty_string x)};
+  name: x:Ter.string_heap_index{not (Te.is_null x) && not (Heap.is_indexing_empty_string string_heap x)};
 
   (* - Mvid (an index into the Guid heap; simply a Guid used to distinguish between two versions of the same module) *)
-  mvid: x:Te.guid_heap_index{not (Te.is_null x) && not (Te.is_indexing_null_guid x)};
+  mvid: x:Ter.guid_heap_index{not (Te.is_null x) && not (Heap.is_indexing_null_guid guid_heap x)};
 }
 //---|
 
@@ -34,8 +38,10 @@ type module_schema = {
 *)
 
 (* The TypeRef table has the following columns: *)
+noeq
 type typeref_schema = {
 
+  string_heap: Heap.string_heap;
   (* 
      - ResolutionScope (an index into a Module, ModuleRef, AssemblyRef or TypeRef table, or null; 
        more precisely, a ResolutionScope coded index) 
@@ -45,11 +51,11 @@ type typeref_schema = {
   resolution_scope: option (x:M.resolution_scope{x <> M.ResolutionScopeModule});
 
   (* 2. TypeName shall index a non-empty string in the String heap [ERROR] *)
-  type_name: x:Te.string_heap_index{not (Te.is_null x) && not (Te.is_indexing_empty_string x)};
+  type_name: x:Ter.string_heap_index{not (Te.is_null x) && not (Heap.is_indexing_empty_string string_heap x)};
 
   (* 3. TypeNamespace can be null, or non-null *)
   (* 4. If non-null, TypeNamespace shall index a non-empty string in the String heap [ERROR] *)
-  type_namespace: x:Te.string_heap_index{Te.is_null x || not (Te.is_indexing_empty_string x)}
+  type_namespace: x:Ter.string_heap_index{Te.is_null x || not (Heap.is_indexing_empty_string string_heap x)}
 }
 
 //---|
